Lp2lc/Next/STLC/__Infer_Umbral.lean
@@ -8,6 +8,17 @@ namespace Umbral
 
 section variable [env : ProvingBase]
 
+/-
+safety condition given only a term
+
+comparing to the safety condition in [__Infer.lean], it is much shorter
+-/
+def Safety [env : ProvingBase]
+    (trm : AST.Trm env.ExeParameters) (typ : AST.Typ env.BuildParameters) : Prop :=
+  trm.eval.isSemiDecidable
+    (λ value => (value.asTrm.map env.ExeParameters env.BuildParameters (Sum.inl) id).CanInhabit typ)
+
+infer_core
 structure SafetyOf (trm : AST.Trm env.BuildParameters) where
   typ : AST.Typ env.BuildParameters
   -- safety : Safety trm typ -- TODO: this lemma has been temporarily disabled. Enable it later.
